test/frontends/alpine.t/run.t
@@ -1,0 +1,8 @@
+  $ ../../../src/main.exe alpine APKINDEX app docs | sed -E '/^(parse|solve) [0-9.]+s$/d'
+  index APKINDEX
+  cone: 3 packages, 0 provide rows, 1 install_if rows
+  packages (3):
+    app 1.0
+    app-doc 1.0
+    docs 1.0
+  encoded solution: 8 core nodes (4 Alpine packages encoded)
